Revise mult example

examples/mult/MultHeader.v
@@ -18,21 +18,22 @@ Set Implicit Arguments.
 
 
 Instance fRA: URA.t := Excl.t Z%ra.
-Instance gRA: URA.t := Excl.t bool%ra.
-Instance hRA: URA.t := Excl.t nat%ra.
+Instance gRA: URA.t := Excl.t nat%ra.
+Instance hRA: URA.t := Excl.t bool%ra.
+Definition fblack: fRA := ε.
 Definition f0: fRA := Some 5%Z.
 Definition f1: fRA := Some 6%Z.
 Definition f2: fRA := Some 7%Z.
 Definition f3: fRA := Some 8%Z.
-Definition gpre: gRA := Some true.
-Definition gpost: gRA := Some false.
-Definition hpre: hRA := Some 15.
-Definition hpost: hRA := Some 17.
+Definition gpre (n: nat): gRA := Some n.
+Definition gpost (n: nat): gRA := Some (n + 1).
+Definition hpre: hRA := Some true.
+Definition hpost: hRA := Some false.
 
-Lemma f01_update: URA.updatable f0 f1.
-Proof. eapply Excl.updatable; et. ur; ss. Qed.
-Lemma f23_update: URA.updatable f2 f3.
-Proof. eapply Excl.updatable; et. ur; ss. Qed.
+Lemma f01_update: URA.updatable (fblack ⋅ f0) (fblack ⋅ f1).
+Proof. eapply URA.updatable_add; try refl. eapply Excl.updatable; et. ur; ss. Qed.
+Lemma f23_update: URA.updatable (fblack ⋅ f2) (fblack ⋅ f3).
+Proof. eapply URA.updatable_add; try refl. eapply Excl.updatable; et. ur; ss. Qed.
 
 Global Opaque f0 f1 f2 f3 gpre gpost hpre hpost.
 
@@ -42,28 +43,30 @@ Section PROOF.
   Context `{@GRA.inG gRA Σ}.
   Context `{@GRA.inG hRA Σ}.
 
-  Definition f_spec0: fspec := mk_simple (fun (_: unit) => (ord_top,
-                                                            (fun varg => (OwnM f1 ** OwnM gpre)%I),
-                                                           (fun vret => (OwnM f2 ** OwnM gpost)%I))).
-  Definition f_spec1: fspec := mk_simple (fun (_: unit) => (ord_top,
-                                                            (fun varg => (OwnM f0 ** OwnM gpre ** OwnM hpre)%I),
-                                                           (fun vret => (OwnM f3 ** OwnM gpost ** OwnM hpost)%I))).
-  Definition g_spec: fspec := mk_simple (fun (_: unit) => (ord_top,
-                                                           (fun varg => (OwnM gpre)%I),
-                                                           (fun vret => (OwnM gpost)%I))).
+  Definition f_spec0: fspec :=
+    mk_simple (fun (n: nat) => (ord_top,
+                                  (fun _ => (OwnM f1 ** OwnM (gpre n))%I),
+                                  (fun _ => (OwnM f2 ** OwnM (gpost n))%I))).
+  Definition f_spec1: fspec :=
+    mk_simple (fun (n: nat) => (ord_top,
+                                  (fun _ => (OwnM f0 ** OwnM (gpre n) ** OwnM hpre)%I),
+                                  (fun _ => (OwnM f3 ** OwnM (gpost n) ** OwnM hpost)%I))).
+  Definition g_spec: fspec := mk_simple (fun (n: nat) => (ord_top,
+                                                           (fun _ => (OwnM (gpre n))%I),
+                                                           (fun _ => (OwnM (gpost n))%I))).
   Definition h_spec0: fspec := fspec_trivial.
   Definition h_spec1: fspec := mk_simple (fun (_: unit) => (ord_top,
-                                                            (fun varg => (OwnM hpre)%I),
-                                                            (fun vret => (OwnM hpost)%I))).
+                                                            (fun _ => (OwnM hpre)%I),
+                                                            (fun _ => (OwnM hpost)%I))).
 
   Definition GlobalStb0: list (gname * fspec).
     eapply (Seal.sealing "stb").
-    apply [("ff", f_spec0); ("f", f_spec0); ("g", g_spec); ("h", h_spec0)].
+    apply [("feasy", f_spec0); ("fhard", f_spec0); ("g", g_spec); ("h", h_spec0)].
   Defined.
 
   Definition GlobalStb1: list (gname * fspec).
     eapply (Seal.sealing "stb").
-    apply [("ff", f_spec0); ("f", f_spec1); ("g", g_spec); ("h", h_spec1)].
+    apply [("feasy", f_spec0); ("fhard", f_spec1); ("g", g_spec); ("h", h_spec1)].
   Defined.
 
   (* Definition GlobalStb0: gname -> option fspec := to_stb [("f", f_spec0); ("g", g_spec); ("h", h_spec0)]. *)
@@ -82,3 +85,14 @@ End PROOF.
 
 Global Hint Unfold GlobalStb0: stb.
 Global Hint Unfold GlobalStb1: stb.
+
+(*** TODO: move to PCM.v ***)
+Lemma GRA_unit: ∀ {A : URA.t} {Σ : GRA.t} {H : GRA.inG A Σ}, GRA.embed (ε: A) = ε.
+Proof.
+ i. destruct H. subst. unfold GRA.embed.
+ Local Transparent GRA.to_URA.
+ unfold GRA.to_URA.
+ cbn.
+ Local Opaque GRA.to_URA.
+ eapply func_ext_dep. i. des_ifs.
+Qed.
