examples/mult/Mult01proof.v
@@ -17,7 +17,7 @@ From ExtLib Require Import
      Data.Map.FMapAList.
 
 Require Import STB ProofMode.
-Require Import HTactics2 ISim2 IProofMode2.
+Require Import HTactics2 HSim2 ISim2 IProofMode2.
 
 Set Implicit Arguments.
 
@@ -37,7 +37,7 @@ Section SIMMODSEM.
     @mk_wf
       _
       unit
-      (fun _ _ st_tgt => ⌜True⌝%I)
+      (fun _ _ st_tgt => OwnM fblack)
   .
 
   Theorem correct: refines2 [Mult0.Mult (fun _ => to_stb GlobalStb0)] [Mult1.Mult (fun _ => to_stb GlobalStb1)].
@@ -45,26 +45,54 @@ Section SIMMODSEM.
     eapply adequacy_local2. econs; ss.
     i. econstructor 1 with (wf:=wf) (le:=top2); ss; et; swap 2 3.
     { esplits. rp; [econs|..]; try refl; cycle 1.
-      { repeat f_equal. rewrite URA.unit_id; ss. }
+      { repeat f_equal. rewrite URA.unit_idl; ss. }
       eapply to_semantic. iIntros "H". iSplits; ss. }
 
     econs; [|ss].
     { econs; r; ss. startproof.
-      i. esplits; eauto.
-      iIntros. iDes. iModIntro. iFrame. iSplits; ss. steps. iIntros. iDes. subst. iFrame; ss.
+      (*** given src aux var, choose tgt aux var ***)
+      intro n. exists n. esplits; eauto.
+      (*** we have "SI * P_src" ***)
+      iIntros. iDes. subst.
+      (*** prove "P_tgt" ***)
+      iModIntro. iFrame. iSplits; ss.
+      (*** and proceed the proof. ***)
+      steps.
+      (*** at the end, prove "Q_tgt -* (Q_src * SI)" ***)
+      iIntros. iDes. iFrame; ss.
     }
 
     econs; [|ss].
     { econs; r; ss. startproof.
       i. esplits; eauto.
-      iIntros. iDes. iFrame. iSplits; ss. iDestruct (OwnM_Upd with "A0") as ">A0".
+      iIntros. iDes. subst. iFrame.
+      (*** It is important that the goal contains update modality in the goal "#=> (P_tgt ∗ ...)".
+           This allows update on (SI * P_src) together, not just P_src. ***)
+      unfold inv_with. iDes.
+      iDestruct (OwnM_Upd with "[A A0]") as ">A0".
       { eapply f01_update. }
-      steps. iIntros. iDes. subst. iFrame; ss. iModIntro. iSplits; et. steps.
-      iSplits; ss. iIntros. iSplits; ss. iIntros; iDes. iFrame. iSplits; ss. iIntros; iDes. subst.
-      iFrame. iSplits; ss. steps. iSplits; ss. iIntros. iSplits; ss. iIntros. iFrame. iSplits; ss.
-      iIntros. iDes; subst. iSplits; ss. steps. iIntros; iDes. iFrame.
-      iDestruct (OwnM_Upd with "A0") as ">A0".
+      { iCombine "A A0" as "A". iFrame. }
+      iDestruct "A0" as "[A A0]".
+      iFrame. iModIntro. iSplits; et.
+
+      (*** when calling a function, given tgt aux var, choose src aux var. ***)
+      steps. iSplits; ss. iIntros. iSplits; ss.
+      (*** we get "Q_tgt" ***)
+      iIntros; iDes.
+      (*** and prove "SI * Q_src * ..." ***)
+      iFrame. iSplits; ss. iIntros; iDes. subst. iFrame. iSplits; ss.
+
+      (*** now calling a function which has different conditions on src/tgt. the rules are the same. ***)
+      steps. iSplits; ss. iIntros. iSplits; ss. iIntros. iFrame. iSplits; ss.
+      iIntros. iDes; subst.
+
+      (*** returning, same as above. ***)
+      iSplits; ss. steps. iIntros; iDes.
+      unfold inv_with. iDes.
+      iDestruct (OwnM_Upd with "[A0 A1]") as ">A1".
       { eapply f23_update. }
+      { iCombine "A0 A1" as "A0". iFrame. }
+      iDestruct "A1" as "[A1 A0]".
       iFrame. iModIntro. iSplits; ss.
     }
 
