examples/mult/Mult1.v
@@ -20,15 +20,15 @@ Section PROOF.
   Context `{@GRA.inG hRA Σ}.
 
   Definition multSbtb: list (gname * fspecbody) :=
-    [("f", mk_specbody f_spec0 (fun _ => Ret Vundef↑));
-    ("ff", mk_specbody f_spec1 (fun _ => `_: val <- ccallU "g" tt;; `_: val <- ccallU "h" tt;; Ret Vundef↑));
+    [("feasy", mk_specbody f_spec0 (fun _ => Ret Vundef↑));
+    ("fhard", mk_specbody f_spec1 (fun _ => `_: val <- ccallU "g" tt;; `_: val <- ccallU "h" tt;; Ret Vundef↑));
     ("apc", mk_specbody f_spec0 (fun _ => _ <- Ret Vundef;;; Ret Vundef↑))
     ].
 
   Definition SMultSem: SModSem.t := {|
     SModSem.fnsems := multSbtb;
     SModSem.mn := "Mult";
-    SModSem.initial_mr := ε;
+    SModSem.initial_mr := GRA.embed fblack;
     SModSem.initial_st := tt↑;
   |}
   .
